cava2/FifoProperties.v
@@ -19,16 +19,22 @@ Require Import Coq.micromega.Lia.
 Require Import Coq.NArith.NArith.
 Require Import Coq.ZArith.ZArith.
 Require Import Coq.Lists.List.
+
 Require Import coqutil.Tactics.Tactics.
+
 Require Import Cava.Util.List.
 Require Import Cava.Util.Nat.
+Require Import Cava.Util.Byte.
 Require Import Cava.Util.Tactics.
+Require Import Cava.Util.If.
+
 Require Import Cava.Types.
 Require Import Cava.Expr.
 Require Import Cava.ExprProperties.
 Require Import Cava.Primitives.
 Require Import Cava.Semantics.
 Require Import Cava.Fifo.
+
 Import ListNotations.
 
 Local Open Scope bool.
@@ -394,4 +400,1014 @@ Section FifoSpec.
   Qed.
 
 End FifoSpec.
+
+
+Section RealignerSpec.
+  Open Scope N.
+
+  Ltac easy_bit_bang n :=
+      repeat (
+        destruct n;
+          [first
+            [ rewrite (N.shiftl_spec_low) by lia;now rewrite Bool.andb_false_r
+             | now rewrite Bool.andb_true_r
+          ]|] ).
+
+  Lemma mask_1000 x:
+    x < 2 ^ 32 -> N.land x 0xFF000000 = N.shiftl (N.shiftr x 24) 24.
+  Proof.
+    clear. intros.
+    apply N.bits_inj.
+    cbv [N.eqf]; intros.
+    rewrite N.land_spec.
+
+    replace n with (N.of_nat (N.to_nat n)) by now rewrite N2Nat.id.
+    remember (N.to_nat n) as n'.
+    clear Heqn' n.
+
+    { easy_bit_bang n'.
+      rewrite N.shiftl_spec_high' by lia.
+      rewrite N.shiftr_spec by lia.
+      easy_bit_bang n'.
+      rewrite N.bits_above_log2.
+      { rewrite Bool.andb_false_l.
+        rewrite N.bits_above_log2.
+        { reflexivity. }
+        apply (N.lt_le_trans _ 32).
+        { destr (x =? 0). { rewrite E. now cbn. }
+          apply N.log2_lt_pow2; lia.
+        }
+        lia.
+      }
+      apply (N.lt_le_trans _ 32).
+      { destr (x =? 0). { rewrite E. now cbn. }
+        apply N.log2_lt_pow2; lia.
+      }
+      lia.
+    }
+  Qed.
+
+  Lemma mask_1100 x:
+    x < 2 ^ 32 -> N.land x 0xFFFF0000 = N.shiftl (N.shiftr x 16) 16.
+  Proof.
+    clear. intros.
+    apply N.bits_inj.
+    cbv [N.eqf]; intros.
+    rewrite N.land_spec.
+
+    replace n with (N.of_nat (N.to_nat n)) by now rewrite N2Nat.id.
+    remember (N.to_nat n) as n'.
+    clear Heqn' n.
+
+    { easy_bit_bang n'.
+      rewrite N.shiftl_spec_high' by lia.
+      rewrite N.shiftr_spec by lia.
+      easy_bit_bang n'.
+      rewrite N.bits_above_log2.
+      { rewrite Bool.andb_false_l.
+        rewrite N.bits_above_log2.
+        { reflexivity. }
+        apply (N.lt_le_trans _ 32).
+        { destr (x =? 0). { rewrite E. now cbn. }
+          apply N.log2_lt_pow2; lia.
+        }
+        lia.
+      }
+
+      apply (N.lt_le_trans _ 32).
+      { destr (x =? 0). { rewrite E. now cbn. }
+        apply N.log2_lt_pow2; lia.
+      }
+
+      lia.
+    }
+  Qed.
+
+  Lemma mask_1110 x:
+    x < 2 ^ 32 -> N.land x 0xFFFFFF00 = N.shiftl (N.shiftr x 8) 8.
+  Proof.
+    clear. intros.
+    apply N.bits_inj.
+    cbv [N.eqf]; intros.
+    rewrite N.land_spec.
+
+    replace n with (N.of_nat (N.to_nat n)) by now rewrite N2Nat.id.
+    remember (N.to_nat n) as n'.
+    clear Heqn' n.
+
+    { easy_bit_bang n'.
+      rewrite N.shiftl_spec_high' by lia.
+      rewrite N.shiftr_spec by lia.
+      easy_bit_bang n'.
+
+      rewrite N.bits_above_log2.
+      { rewrite Bool.andb_false_l.
+        rewrite N.bits_above_log2.
+        { reflexivity. }
+        apply (N.lt_le_trans _ 32).
+        { destr (x =? 0). { rewrite E. now cbn. }
+          apply N.log2_lt_pow2; lia.
+        }
+        lia.
+      }
+
+      apply (N.lt_le_trans _ 32).
+      { destr (x =? 0). { rewrite E. now cbn. }
+        apply N.log2_lt_pow2; lia.
+      }
+
+      lia.
+    }
+  Qed.
+
+  Lemma fold_left_4_byte_suffix x xs:
+    (length xs = 4)%nat ->
+    exists e: {X:N | X < 2 ^ 32},
+    (fold_left
+       (fun (acc : N) (b3 : Byte.byte) => N.lor (N.shiftl acc 8) (Byte.to_N b3))
+       xs x)
+    = N.lor (N.shiftl x 32) (proj1_sig e).
+  Proof.
+    intros.
+    destruct xs; [easy|].
+    destruct xs; [easy|].
+    destruct xs; [easy|].
+    destruct xs; [easy|].
+    destruct xs; [|easy].
+    eexists (x:= exist (fun n => n < 2 ^ 32)
+       (N.lor
+       (N.lor
+          (N.lor (N.shiftl (N.shiftl (N.shiftl (Byte.to_N b) 8) 8) 8)
+             (N.shiftl (N.shiftl (Byte.to_N b0) 8) 8))
+          (N.shiftl (Byte.to_N b1) 8)) (Byte.to_N b2))
+        _
+    ).
+    cbn.
+    intros.
+    apply N.bits_inj; cbv [N.eqf]; intros.
+    push_Ntestbit.
+    destr (n <? 32).
+    { rewrite N.shiftl_spec_low with (n:=32) by lia.
+      destr (n <? 8).
+      { push_Ntestbit. shelve. }
+      { push_Ntestbit.
+        destr (n <? 16).
+        { rewrite N.shiftl_spec_low.
+          { shelve. }
+          { lia. }
+        }
+        push_Ntestbit.
+        destr (n <? 24).
+        { rewrite N.shiftl_spec_low.
+          { shelve. }
+          { lia. }
+        }
+        push_Ntestbit.
+        repeat rewrite Bool.orb_false_l.
+        repeat rewrite <- N.shiftl_spec_high by lia.
+        repeat rewrite <- N.lor_spec.
+        reflexivity.
+      }
+    }
+    push_Ntestbit.
+    repeat rewrite testbit_byte by lia.
+    repeat rewrite <- N.sub_add_distr.
+    repeat rewrite Bool.orb_false_r.
+    cbn.
+    reflexivity.
+
+    Unshelve.
+    { repeat rewrite N.shiftl_shiftl.
+      cbn.
+      change 4294967296 with (2^32).
+
+      repeat (
+        change (2^32) with (N.max (2^32) (2^32));
+        apply N.lor_lt);
+        try rewrite N.shiftl_mul_pow2.
+
+        { apply (N.lt_le_trans _ (2 ^ 8 * 2 ^ 24)); try (cbn; lia).
+          { apply N.mul_lt_mono_pos_r. { now cbn. }
+            cbn.
+            pose (Byte.to_N_bounded b).
+            lia.
+          }
+        }
+        { apply (N.lt_le_trans _ (2 ^ 8 * 2 ^ 16)); try (cbn; lia).
+          { apply N.mul_lt_mono_pos_r. { now cbn. }
+            cbn.
+            pose (Byte.to_N_bounded b0).
+            lia.
+          }
+        }
+        { apply (N.lt_le_trans _ (2 ^ 8 * 2 ^ 8)); try (cbn; lia).
+          { apply N.mul_lt_mono_pos_r. { now cbn. }
+            cbn.
+            pose (Byte.to_N_bounded b1).
+            lia.
+          }
+        }
+        pose (Byte.to_N_bounded b2).
+        cbn; lia.
+    }
+
+    all: push_Ntestbit;
+         repeat rewrite Bool.orb_false_l; reflexivity.
+  Qed.
+
+  Lemma shiftr_concat_bytes_4 (x: list Byte.byte):
+    (length x < 8)%nat ->
+    N.shiftr (BigEndianBytes.concat_bytes (List.resize Byte.x00 8 x)) (N.of_nat 32) =
+    BigEndianBytes.concat_bytes (List.resize Byte.x00 4 x).
+  Proof.
+    cbv [BigEndianBytes.concat_bytes].
+    intros.
+    Ltac t :=
+      cbn -[N.shiftr ];
+      repeat rewrite N.lor_0_r;
+      repeat rewrite N.shiftl_shiftl;
+      try rewrite N.shiftr_shiftl_l by lia;
+      try rewrite N.shiftl_0_r;
+      try now cbn.
+    destruct x; [t|
+    destruct x; [t|
+    destruct x; [t|
+    destruct x; [t|]]]].
+
+    repeat rewrite resize_cons.
+    cbn [fold_left].
+    pose (fold_left_4_byte_suffix
+       (N.lor
+          (N.shiftl
+             (N.lor
+                (N.shiftl
+                   (N.lor (N.shiftl (N.lor (N.shiftl 0 8) (Byte.to_N b)) 8)
+                      (Byte.to_N b0)) 8) (Byte.to_N b1)) 8)
+          (Byte.to_N b2))
+        (List.resize Byte.x00 4 x)
+    ).
+    destruct e.
+    { apply resize_length. }
+    rewrite H0.
+    cbn -[N.shiftr].
+    rewrite N.shiftr_lor.
+    rewrite N.shiftr_shiftl_l by lia.
+    assert (N.shiftr (@proj1_sig N (fun X : N => (X < 4294967296)%N) x0) 32 = 0%N).
+    { rewrite N.shiftr_eq_0; [reflexivity|].
+      destruct x0.
+      cbn [proj1_sig].
+      destr (x0 =? 0)%N.
+      { rewrite E. now cbn. }
+      apply N.log2_lt_pow2.
+      { lia. }
+      apply l.
+    }
+    rewrite H1.
+    rewrite N.lor_0_r.
+    rewrite N.shiftl_0_r.
+    reflexivity.
+  Qed.
+
+  Lemma bytes_to_N_id_4 xs:
+    BigEndianBytes.N_to_bytes 4 (BigEndianBytes.concat_bytes (List.resize Byte.x00 4 xs)) = xs.
+  Admitted.
+
+  Lemma concat_bytes_4_bound xs: 
+    BigEndianBytes.concat_bytes (List.resize Byte.x00 4 xs) < 2 ^ 32.
+  Admitted.
+
+  Lemma concat_bytes_8_bound xs: 
+    BigEndianBytes.concat_bytes (List.resize Byte.x00 8 xs) < 2 ^ 64.
+  Admitted.
+
+  Lemma concat_bytes_skip_4_of_8_spec xs n:
+      (length xs < 8)%nat -> 
+      n < 32 ->
+        N.testbit
+          (BigEndianBytes.concat_bytes (List.resize Byte.x00 8 (skipn 4 xs))) n = false.
+  Admitted.
+
+  Lemma concat_bytes_lower_8_zero xs n:
+      (length xs < 4)%nat -> 
+      n < 32 ->
+        N.testbit
+          (BigEndianBytes.concat_bytes (List.resize Byte.x00 8 xs)) n = false.
+  Admitted.
+
+  Lemma concat_bytes_skip_lower_is_upper xs n:
+        32 <= n -> n < 64 ->
+        N.testbit (BigEndianBytes.concat_bytes (List.resize Byte.x00 8 xs))
+          (n - 32) =
+        N.testbit
+          (BigEndianBytes.concat_bytes (List.resize Byte.x00 8 (skipn 4 xs)))
+          n.
+  Admitted.
+
+  Lemma concat_bytes_8_is_64bit xs n:
+        64 <= n -> 
+        N.testbit
+          (BigEndianBytes.concat_bytes (List.resize Byte.x00 8 xs))
+          n = false.
+  Admitted.
+
+  Lemma length_N_to_byte n xs:
+          length (BigEndianBytes.N_to_bytes n xs) = n.
+  Admitted.
+
+  Lemma concat_bytes_truncation x:
+    (N.shiftr
+      (BigEndianBytes.concat_bytes (List.resize Byte.x00 8 x))
+      (N.of_nat 32) mod 2 ^ N.of_nat 32)%N 
+      = BigEndianBytes.concat_bytes (List.resize Byte.x00 4 x).
+  Admitted.
+
+  Definition realign_inner_spec
+    (existing: list Byte.byte) data data_mask := (
+      let '(a,b,c,d) :=
+        match BigEndianBytes.N_to_bytes 4 data with
+        | a::b::c::d::_ => (a,b,c,d)
+        | _ => (Byte.x00,Byte.x00,Byte.x00,Byte.x00)
+        end in
+      existing ++
+           if data_mask =? 0x0 then []
+      else if data_mask =? 0x1 then [d]
+      else if data_mask =? 0x2 then [c]
+      else if data_mask =? 0x4 then [b]
+      else if data_mask =? 0x8 then [a]
+      else if data_mask =? 0x3 then [c;d]
+      else if data_mask =? 0x6 then [b;c]
+      else if data_mask =? 0xC then [a;b]
+      else if data_mask =? 0x9 then [b;c;d]
+      else if data_mask =? 0xE then [a;b;c]
+      else [a;b;c;d]
+      )%N.
+
+  Definition realign_inner_pre
+    existing'
+    (input : denote_type (input_of (realign_inner (var:=denote_type) )))
+    :=
+    let '(existing, (existing_len, (data, (data_mask, tt)))) := input in
+    existing < 2 ^ 32 /\
+    existing_len < 4 /\
+    data < 2 ^ 32 /\
+    existing' = (firstn (N.to_nat existing_len) (BigEndianBytes.N_to_bytes 4 existing)).
+
+  Lemma step_realign_inner
+    existing'
+    (input : denote_type (input_of (realign_inner (var:=denote_type) )))
+    (state : denote_type (state_of (realign_inner (var:=denote_type) ))):
+    realign_inner_pre existing' input ->
+    step realign_inner state input =
+    let aligned := realign_inner_spec existing' (fst (snd (snd input))) (fst (snd (snd (snd input)))) in
+    (tt, (BigEndianBytes.concat_bytes (List.resize Byte.x00 8 aligned), N.of_nat (length aligned))).
+  Proof.
+    destruct input as (existing, (existing_len, (input, (input_mask, [])))).
+    cbn in state.
+    cbv [realign_inner realign_inner_pre realign_inner_spec K bvconcat bvslice bvresize] in *;
+      stepsimpl.
+    repeat (destruct_pair_let; cbn[fst snd]).
+    intros Hpre.
+    destruct Hpre as [? [? [? ?]]].
+    rewrite H2 in *.
+
+    f_equal.
+
+    cbv [BigEndianBytes.N_to_bytes seq List.map].
+
+    cbn [Nat.add].
+    repeat rewrite N.lor_0_r.
+    repeat rewrite N.land_ones.
+
+    do 4 rewrite mask_1000 by (try apply N.mod_upper_bound; lia).
+    do 3 rewrite mask_1100 by (try apply N.mod_upper_bound; lia).
+    do 2 rewrite mask_1110 by (try apply N.mod_upper_bound; lia).
+
+    repeat
+      match goal with
+      | |- context [N.eqb existing_len ?X] =>
+        let H := fresh in destruct (N.eqb_spec existing_len X) as [H|H]; try rewrite H
+      | |- context [N.eqb input_mask ?X] =>
+        let H := fresh in destruct (N.eqb_spec input_mask X) as [H|H]; try rewrite H
+      end;
+      try match goal with
+      | _: ?X <> 0
+      , _: ?X <> 1
+      , _: ?X <> 2
+      , _: ?X < 4
+      |- _ =>
+        let H := fresh in
+        assert (X = 3) by lia; rewrite H
+      end.
+
+    all:
+      f_equal;
+      try rewrite app_nil_r;
+      try rewrite length_app;
+      try rewrite firstn_length;
+      cbv [firstn N.to_nat Pos.to_nat Pos.iter_op Nat.add];
+      cbv [BigEndianBytes.concat_bytes repeat List.resize fold_left List.app fst snd length Nat.sub Init.Nat.min N.of_nat firstn];
+      repeat rewrite N2Byte.id;
+      cbv [Byte.to_N];
+      repeat rewrite N.lor_0_r;
+      repeat rewrite N.shiftl_shiftl;
+      repeat rewrite N.div2_spec;
+      repeat rewrite N.shiftr_shiftr;
+      cbn [fst snd Nat.add Nat.sub N.add Pos.add Pos.succ Pos.of_succ_nat].
+
+    Ltac brute :=
+      repeat (first
+        [
+          rewrite Bool.orb_false_l
+        | rewrite Bool.orb_false_r
+        | rewrite N.shiftl_spec_low by lia
+        | rewrite N.mod_pow2_bits_low by lia
+        | rewrite N.shiftl_spec_high by lia
+        | rewrite N.mod_pow2_bits_high by lia
+        | rewrite N.shiftr_spec by lia
+        | rewrite N.shiftl_0_l by lia
+        | rewrite N.shiftl_0_r by lia
+        | rewrite N.lor_0_l by lia
+        | rewrite N.lor_0_r by lia
+        | rewrite N.shiftr_0_l by lia
+        | rewrite N.shiftr_0_r by lia
+        | rewrite N.lor_spec by lia
+        ]);
+        try reflexivity;
+        try match goal with
+            | |- N.testbit ?i ?X = N.testbit ?i ?Y => f_equal; lia
+            end;
+        try lia.
+
+    all:
+      apply N.bits_inj; cbv [N.eqf]; intros;
+
+      change (0*8) with 0;
+      change (256) with (2^8);
+
+      destr (n <? 64); brute;
+      destr (n <? 32); brute;
+      destr (n <? 24); brute;
+      destr (n <? 56); brute;
+      destr (n <? 48); brute;
+      destr (n <? 16); brute;
+      destr (n <? 40); brute;
+      destr (n <? 8); brute.
+
+    all:
+      rewrite N.testbit_high_lt with (x:=input) (n:=32) by lia;
+      rewrite Bool.orb_false_r;
+      match goal with
+      | |- N.testbit ?i ?X = N.testbit ?i ?Y => f_equal; lia
+      end.
+  Qed.
+
+  Definition realign_spec
+    latched_valid
+    latched_bytes
+    state_data
+    (input : denote_type (input_of (var:=denote_type) realign)) := (
+    let '(_, (_, (_, (flush, (consumer_ready, tt))))) := input in
+
+    if negb consumer_ready then
+      (latched_valid, (BigEndianBytes.concat_bytes (List.resize Byte.x00 4 latched_bytes), N.of_nat (length latched_bytes)))
+    else
+      let out := firstn 4 state_data in
+      let valid := 4 <=? length state_data in
+
+      let valid_or_flushing := valid || (flush && (1 <=? length state_data)) in
+
+      (valid_or_flushing, (BigEndianBytes.concat_bytes (List.resize Byte.x00 4 out), N.of_nat (length out))))%nat.
+
+  Definition realign_update_state
+    state_data
+    (input : denote_type (input_of (var:=denote_type) realign)) := (
+    let '(data_valid, (data, (data_mask, (flush, (consumer_ready, tt))))) := input in
+    if negb consumer_ready then
+      state_data
+    else
+      let state' :=
+        if (4 <=? length state_data) || flush then
+          skipn 4 state_data
+        else state_data in
+
+      if data_valid && negb flush then realign_inner_spec state' data data_mask else state')%nat.
+
+  Definition realign_update_latched_bytes
+    (latched_bytes: list Byte.byte)
+    state_data
+    (input : denote_type (input_of (var:=denote_type) realign))
+    :=
+    let '(data_valid, (data, (data_mask, (flush, (consumer_ready, tt))))) := input in
+    if negb consumer_ready then
+      latched_bytes
+    else
+      firstn 4 state_data.
+
+  Definition realign_update_latched_valid
+    (latched_valid: bool)
+    (state_data: list Byte.byte)
+    (input : denote_type (input_of (var:=denote_type) realign)) := (
+    let '(data_valid, (data, (data_mask, (flush, (consumer_ready, tt))))) := input in
+    if negb consumer_ready then
+      latched_valid
+    else
+      (4 <=? length state_data) || flush && (1 <=? length state_data))%nat.
+
+  Definition realign_pre
+    (input : denote_type (input_of (var:=denote_type) realign))
+    (state: denote_type (state_of (var:=denote_type) realign))
+    :=
+    let '(data_valid, (data, (data_mask, (flush, (consumer_ready, tt))))) := input in
+
+    (data < 2 ^ 32)%N
+    .
+
+  Definition realign_invariant
+    latched_valid latched_bytes
+    (ghost_state: list Byte.byte)
+    (state: denote_type (state_of (var:=denote_type) realign))
+    :=
+    let '(out_valid, (out_data, (out_len, (buff, buff_len)))) := state in
+
+    buff_len = N.of_nat (length ghost_state)
+    (* buff_len = N.of_nat (length (firstn 4 ghost_state)) *)
+    /\ out_valid = latched_valid
+    /\ out_data = BigEndianBytes.concat_bytes (List.resize Byte.x00 4 latched_bytes)
+    /\ N.to_nat out_len = length latched_bytes
+    (* /\ True *)
+    /\ buff = BigEndianBytes.concat_bytes (List.resize Byte.x00 8 ghost_state)
+    (* /\ N.shiftr buff (N.of_nat 32) = BigEndianBytes.concat_bytes (firstn 4 ghost_state) *)
+    /\ (buff < 2 ^ 64)%N
+    /\ (buff_len < 8)%N
+    .
+
+
+  Lemma step_realign_invariant
+    latched_valid latched_bytes state_data
+    next_latched_valid next_latched_bytes next_state_data
+      (input : denote_type (input_of (realign (var:=denote_type) )))
+      (state : denote_type (state_of (realign (var:=denote_type) ))) :
+    next_state_data = realign_update_state state_data input ->
+    next_latched_bytes = realign_update_latched_bytes latched_bytes state_data input ->
+    next_latched_valid = realign_update_latched_valid latched_valid state_data input ->
+    realign_pre input state ->
+    realign_invariant latched_valid latched_bytes state_data state ->
+    realign_invariant next_latched_valid next_latched_bytes next_state_data (fst (step realign state input)).
+  Proof.
+    destruct input as (input_valid, (input_data, (input_mask, (flush, (consumer_ready, []))))).
+    destruct state as (out_valid, (out_data, (out_length, (q, q_len)))).
+    intros Hst Hlatch Hlatchvalid Hpre Hinv.
+    destruct Hinv as [Hbuff_len [Hlatch_valid [Hlatch_bytes [Hlatch_bytes_len [Hfirst_bytes [Hbuf_bound Hbuf_len_bound]]]]]].
+(* bvresize bvconcat bvmin bvslice *)
+    cbv [realign realign_spec realign_pre realign_invariant realign_update_state realign_update_latched_bytes realign_update_latched_valid K] in *;
+    stepsimpl.
+
+    repeat (destruct_pair_let; cbn[fst snd]);
+    autorewrite with tuple_if.
+    erewrite step_realign_inner.
+
+    2: {
+      cbv [realign_inner_pre].
+      split.
+      { cbv [bvslice bvresize]; stepsimpl; cbn [fst snd].
+        destruct ( (4 <=? q_len) || flush)%N;
+        rewrite N.land_ones; replace (N.of_nat 32) with 32%N by lia;
+        apply N.mod_lt; try lia.
+      }
+      split.
+      { cbn [fst snd].
+        destruct ( (4 <=? q_len) )%N eqn:?; boolsimpl.
+        {
+          replace (2^N.of_nat 4)%N with 16%N by now cbn.
+          rewrite N.add_sub_swap by now apply N.leb_le.
+          rewrite N.add_mod by lia.
+          rewrite N.mod_same by lia.
+          rewrite N.add_0_r.
+          rewrite N.mod_mod by lia.
+
+          rewrite N.mod_small.
+          { apply (N.lt_le_trans _ (8 - 4)%N); lia. }
+          lia.
+        }
+        Search (_ <=? _ = false)%N.
+        apply N.leb_gt in Heqb.
+        destruct flush; try lia.
+      }
+      split; [lia|]. reflexivity.
+    }
+
+    autorewrite with tuple_if.
+    destr consumer_ready; cbn [negb fst snd] in *.
+    2: {
+      subst.
+      rewrite Hlatch_bytes_len.
+      tauto.
+    }
+
+
+    assert
+      ((N.of_nat (Init.Nat.min
+                  (N.to_nat
+                     (if (4 <=? N.of_nat (length state_data)) || flush
+                      then
+                       if 4 <=? N.of_nat (length state_data)
+                       then
+                        (N.of_nat (length state_data) + 2 ^ N.of_nat 4 - 4)
+                        mod 2 ^ N.of_nat 4
+                       else 0
+                      else N.of_nat (length state_data))) 4))%N
+        =
+            ((if (4 <=? length state_data)%nat || flush
+              then N.of_nat (length state_data - 4)
+              else N.of_nat (length state_data)) )%N)
+              as Heq1.
+    {  destr ((4 <=? N.of_nat (length state_data)));
+       destr ((4 <=? length state_data))%nat;
+       destruct flush; boolsimpl; try lia; rewrite Nat.min_l;
+           rewrite N.add_sub_swap by apply E;
+           rewrite N.add_mod by (now cbn);
+           rewrite N.mod_same by (now cbn);
+           rewrite N.add_0_r;
+           rewrite N.mod_mod by (now cbn);
+           rewrite N.mod_small; cbn; lia.
+    }
+
+    assert ((
+            if (4 <=? N.of_nat (length state_data))%N || flush
+            then
+             if (4 <=? N.of_nat (length state_data))%N
+             then
+              ((N.of_nat (length state_data) + 2 ^ N.of_nat 4 - 4) mod 2 ^ N.of_nat 4)%N
+             else 0%N
+             else N.of_nat (length state_data)) =
+            (
+            if (4 <=? length state_data) || flush
+            then N.of_nat (length state_data - 4)
+            else N.of_nat (length state_data)))%nat as Heq2.
+    {  destr ((4 <=? N.of_nat (length state_data)));
+       destr ((4 <=? length state_data))%nat;
+       destruct flush; boolsimpl; try lia;
+           rewrite N.add_sub_swap by apply E;
+           rewrite N.add_mod by (now cbn);
+           rewrite N.mod_same by (now cbn);
+           rewrite N.add_0_r;
+           rewrite N.mod_mod by (now cbn);
+           rewrite N.mod_small; cbn; lia.
+    }
+
+    ssplit.
+    {
+      subst; cbn [negb fst snd].
+      autorewrite with tuple_if.
+      cbv [realign_inner_spec].
+      repeat rewrite unfold_N_to_bytes_4.
+      push_length.
+      repeat rewrite Nat2N.of_nat_if.
+      repeat rewrite Nat2N.inj_add.
+      repeat rewrite Nat2N.of_nat_if.
+      rewrite Heq1.
+      rewrite Heq2.
+
+      reflexivity.
+    }
+    {
+      subst;
+      destr (1 <=? length state_data)%nat;
+      destr (1 <=? N.of_nat (length state_data))%N;
+      destr (4 <=? length state_data)%nat;
+      destr (4 <=? N.of_nat (length state_data))%N;
+      try lia; now boolsimpl.
+    }
+    { subst; cbv [bvslice bvresize]; stepsimpl; cbn [fst snd].
+      rewrite N.land_ones_low.
+      { rewrite resize_firstn by lia.
+        now rewrite shiftr_concat_bytes_4 by lia.
+      }
+
+      apply (N.lt_le_trans _ (N.log2 (N.shiftr (2 ^ 64) (N.of_nat 32)))).
+      { compute_expr (N.log2 (N.shiftr (2 ^ 64) (N.of_nat 32)))%N.
+        destr (N.shiftr
+          (BigEndianBytes.concat_bytes (List.resize Byte.x00 8 state_data))
+          (N.of_nat 32)).
+        { cbn; lia. }
+        apply N.log2_lt_pow2.
+        { lia. }
+        rewrite <- E.
+        change (N.of_nat 32) with 32%N.
+        replace (N.shiftr (BigEndianBytes.concat_bytes (List.resize Byte.x00 8 state_data)) 32)
+          with ((BigEndianBytes.concat_bytes (List.resize Byte.x00 8 state_data)) / 2 ^ 32)%N
+          by now rewrite N.shiftr_div_pow2.
+        { apply N.div_lt_upper_bound.
+          { lia. }
+          { now change (2 ^ 32 * 2 ^ 32)%N with (2^64)%N. }
+        }
+      }
+      now cbn.
+    }
+    { subst; cbv [bvmin bvslice bvresize]; stepsimpl; cbn [fst snd].
+      rewrite apply_if_ext_1.
+      repeat rewrite N.land_ones_low.
+      {
+        rewrite firstn_length.
+        destr (N.of_nat (length state_data) <=? 4)%N;
+        destr (length state_data <=? 4)%nat; try lia.
+      }
+      { now cbn. }
+      { change 8%N with (2^3)%N in Hbuf_len_bound.
+        apply (N.lt_trans _ 3).
+        { destr ((0 =? N.of_nat (length state_data))%N).
+          { now rewrite <- E. }
+          { apply N.log2_lt_pow2;lia. }
+        }
+        lia.
+      }
+    }
+    { cbv [bvslice bvresize]; stepsimpl; cbn [fst snd].
+      subst.
+      rewrite Heq2.
+      autorewrite with tuple_if.
+      cbn [fst snd].
+      destruct (input_valid && negb flush).
+      { do 3 f_equal.
+        destr ( (4 <=? length state_data) )%nat;
+        destr ( (4 <=? N.of_nat (length state_data)) )%N;
+        try lia; boolsimpl.
+        { rewrite N.shiftr_0_r.
+          destruct state_data; [cbn in E; contradiction|].
+          destruct state_data; [cbn in E; contradiction|].
+          destruct state_data; [cbn in E; contradiction|].
+          destruct state_data; [cbn in E; contradiction|].
+          destruct state_data. { now cbn. }
+          destruct state_data.
+
+          Local Ltac bitify :=
+            apply Byte2N.inj; rewrite N2Byte.id; apply N.bits_inj; cbv [N.eqf].
+
+          Local Ltac s1 :=
+            rewrite <- N.land_ones with (n:=8);
+            replace 4294967295 with (N.ones 32) by now cbn;
+            push_Ntestbit.
+          Local Ltac s2 :=
+              repeat (rewrite <- N.add_sub_assoc by lia; cbn);
+              repeat rewrite N.add_0_r;
+              repeat match goal with
+                     | |- context [ N.testbit (Byte.to_N _ ) (?x + ?y)] =>
+                      repeat rewrite testbit_byte with (n:= x + y) by lia; boolsimpl
+                     end.
+          Local Ltac s3 :=
+            try reflexivity;
+            try (now apply testbit_byte);
+            try (symmetry; now apply testbit_byte).
+
+          { cbn -[N.shiftr].
+            replace (Pos.to_nat 1) with 1%nat by now cbn.
+            rewrite firstn_cons.
+            rewrite firstn_O.
+            f_equal.
+            bitify; intros; s1.
+            destr (n <? 8);
+              push_Ntestbit;
+              boolsimpl; s2; s3.
+          }
+
+          destruct state_data.
+          { cbn -[N.shiftr].
+            replace (Pos.to_nat 2) with 2%nat by now cbn.
+            repeat rewrite firstn_cons.
+            rewrite firstn_O.
+            f_equal; [|f_equal];
+              bitify; intros; s1;
+              destr (n <? 8);
+                push_Ntestbit;
+                boolsimpl; s2; s3.
+          }
+          destruct state_data.
+          { cbn -[N.shiftr].
+            replace (Pos.to_nat 3) with 3%nat by now cbn.
+            repeat rewrite firstn_cons.
+            rewrite firstn_O.
+            f_equal; [|f_equal;[|f_equal]];
+              bitify; intros; s1;
+              destr (n <? 8);
+                push_Ntestbit;
+                boolsimpl; s2; s3.
+          }
+          cbn in Hbuf_len_bound.
+          lia.
+        }
+        rewrite skipn_all2 by lia.
+        destruct flush.
+        { rewrite Nat2N.id.
+          replace (length state_data - 4)%nat with 0%nat by lia.
+          now rewrite firstn_O.
+        }
+        rewrite shiftr_concat_bytes_4 by lia.
+        rewrite N.land_ones_low by (
+            destr (BigEndianBytes.concat_bytes (List.resize Byte.x00 4 state_data) =? 0);
+            try (rewrite E1; cbn; lia);
+            rewrite <- N.log2_lt_pow2 by lia;
+            now apply concat_bytes_4_bound).
+        rewrite bytes_to_N_id_4.
+        rewrite Nat2N.id.
+        now rewrite firstn_all.
+      }
+
+
+      destr ( (4 <=? length state_data) )%nat;
+      destr ( (4 <=? N.of_nat (length state_data)) )%N;
+      try lia; boolsimpl;
+      apply N.bits_inj; cbv [N.eqf]; intros; push_Ntestbit; boolsimpl.
+      {
+        destr (n <? 32); push_Ntestbit; boolsimpl.
+        { now rewrite concat_bytes_skip_4_of_8_spec by lia. }
+        destr (n <? 64); push_Ntestbit; boolsimpl.
+        {
+          replace (n - N.of_nat 32 + N.of_nat 0) with (n - 32) by lia.
+          now rewrite concat_bytes_skip_lower_is_upper by lia.
+        }
+        now rewrite concat_bytes_8_is_64bit by lia.
+      }
+      {
+        destr (n <? 32); push_Ntestbit; boolsimpl.
+        {
+          destruct flush.
+          { now rewrite concat_bytes_skip_4_of_8_spec by lia. }
+          { now rewrite concat_bytes_lower_8_zero by lia. }
+        }
+        destruct flush;
+        destr (n <? 64); push_Ntestbit; boolsimpl;
+        replace (n - N.of_nat 32 + N.of_nat 0) with (n - 32) by lia.
+        { now rewrite concat_bytes_skip_lower_is_upper by lia. }
+        { now rewrite concat_bytes_8_is_64bit. }
+        { now replace (n - N.of_nat 32 + N.of_nat 32) with n by lia. }
+        now rewrite concat_bytes_8_is_64bit.
+      }
+    }
+    { cbv [bvslice bvresize]; subst; stepsimpl;
+      rewrite Heq2;
+      autorewrite with tuple_if;
+      cbn [fst snd].
+      destruct (input_valid && negb flush).
+      { apply concat_bytes_8_bound. }
+      rewrite N.land_0_l.
+      rewrite N.shiftr_0_r.
+      apply (N.lt_le_trans _ (N.max (2^64) (2^64))).
+      2:{ lia. }
+      apply N.lor_lt with (xs:=64) (ys:=64).
+      2:{ lia. }
+      rewrite N.shiftl_mul_pow2.
+      apply (N.lt_le_trans _ (2^32 * 2^32)).
+      2:{ cbn; lia. }
+      apply N.mul_lt_mono_pos_r.
+      { lia. }
+      Search (N.land).
+      rewrite N.land_ones.
+      apply N.mod_upper_bound.
+      lia.
+    }
+
+    {
+      rewrite Hbuff_len.
+      autorewrite with tuple_if;
+      cbn [fst snd negb].
+      destr (input_valid);
+      destr (flush);
+      destr (4 <=? length state_data)%nat;
+      destr (4 <=? N.of_nat (length state_data))%N;
+      boolsimpl; try lia.
+
+      { rewrite N.add_sub_swap by lia.
+        cbn [N.of_nat].
+        replace (2 ^ 4)%N with (1 * 2 ^ 4)%N at 1 by lia.
+        rewrite N.mod_add by now cbn.
+        rewrite N.mod_small; cbn; lia.
+      }
+      { rewrite N.add_sub_swap by lia.
+        replace (2 ^ 4)%N with (1 * 2 ^ 4)%N at 1 by lia.
+        rewrite N.mod_add by now cbn.
+        rewrite N.mod_small by ( cbn; subst; lia ).
+        rewrite N.shiftr_0_r.
+        cbv [realign_inner_spec ]; subst; stepsimpl;
+        autorewrite with tuple_if;
+        cbn [fst snd]; rewrite unfold_N_to_bytes_4.
+        push_length.
+        replace input_mask with (N.of_nat (N.to_nat input_mask)) by apply N2Nat.id.
+        remember (N.to_nat input_mask) as x.
+        do 14 (destruct x; [cbn; lia|]).
+        repeat match goal with
+        | |- context [?X =? ?Y] => destr (X =? Y); try lia
+        end.
+      }
+      {
+        cbv [realign_inner_spec ]; subst; stepsimpl;
+        autorewrite with tuple_if;
+        cbn [fst snd]; rewrite unfold_N_to_bytes_4.
+        push_length.
+        replace input_mask with (N.of_nat (N.to_nat input_mask)) by apply N2Nat.id.
+        remember (N.to_nat input_mask) as x.
+        do 14 (destruct x; [cbn; lia|]).
+        repeat match goal with
+        | |- context [?X =? ?Y] => destr (X =? Y); try lia
+        end.
+      }
+      { rewrite N.add_sub_swap by lia.
+        replace (2 ^ 4)%N with (1 * 2 ^ 4)%N at 1 by lia.
+        rewrite N.mod_add by now cbn.
+        rewrite N.mod_small; cbn; lia.
+      }
+      { rewrite N.add_sub_swap by lia.
+        cbn [N.of_nat].
+        replace (2 ^ 4)%N with (1 * 2 ^ 4)%N at 1 by lia.
+        rewrite N.mod_add by now cbn.
+        rewrite N.mod_small; cbn; lia.
+      }
+    }
+  Qed.
+
+  Lemma step_realign
+    latched_valid
+    latched_bytes
+      state_data
+      (input : denote_type (input_of (realign (var:=denote_type) )))
+      (state : denote_type (state_of (realign (var:=denote_type) ))) :
+    realign_pre input state ->
+    realign_invariant latched_valid latched_bytes state_data state ->
+    snd (step realign state input) = realign_spec latched_valid latched_bytes state_data input.
+  Proof.
+    destruct input as (input_valid, (input_data, (input_mask, (flush, (consumer_ready, []))))).
+    destruct state as (out_valid, (out_data, (out_length, (q, q_len)))).
+    intros Hpre Hinv.
+
+    destruct Hinv as [Hbuff_len [Hlatch_valid [Hlatch_bytes [Hlatch_bytes_len [Hfirst_bytes Hbuf_bound]]]]].
+    subst.
+
+    cbv [realign realign_spec realign_pre realign_invariant realign_update_state K] in *.
+    stepsimpl.
+
+    repeat (destruct_pair_let; cbn[fst snd]).
+    autorewrite with tuple_if.
+    erewrite step_realign_inner.
+    {
+      cbn [fst snd].
+      rewrite <- Hlatch_bytes_len.
+      rewrite N2Nat.id.
+      cbv [bvslice bvresize bvmin].
+      stepsimpl.
+      rewrite resize_firstn by lia.
+      rewrite N.land_ones.
+      rewrite N.land_ones.
+      rewrite concat_bytes_truncation.
+
+      replace
+        ((if N.of_nat (length state_data) <=? 4
+          then N.of_nat (length state_data)
+          else 4) mod 2 ^ N.of_nat 4)%N with
+          (N.of_nat (length (firstn 4 state_data))).
+      2:{
+        destr (length state_data <=? 4)%nat;
+        destr (N.of_nat (length state_data) <=? 4); try lia.
+        { rewrite firstn_length.
+          rewrite Nat.min_r by lia.
+          now rewrite N.mod_small by (cbn;lia).
+        }
+        { rewrite firstn_length.
+          rewrite Nat.min_l by lia.
+          now rewrite N.mod_small by (cbn;lia).
+        }
+      }
+
+      destr (1 <=? length state_data)%nat;
+      destr (1 <=? N.of_nat (length state_data));
+      destr (4 <=? length state_data)%nat;
+      destr (4 <=? N.of_nat (length state_data)); try lia;
+      reflexivity.
+    }
+    cbn [realign_inner_pre].
+    ssplit.
+    {
+      cbv [bvslice bvresize bvmin].
+      stepsimpl.
+      repeat rewrite N.land_ones.
+      destruct ((4 <=? N.of_nat (length state_data)) || flush)%N;
+      apply N.mod_upper_bound; lia.
+    }
+    {
+      cbv [bvslice bvresize bvmin].
+      stepsimpl.
+      destr (4 <=? length state_data)%nat;
+      destr (4 <=? N.of_nat (length state_data))%N;
+      try lia.
+      {
+        rewrite N.add_sub_swap by lia.
+        replace 16%N with (1*16)%N at 1 by lia. rewrite N.mod_add by now cbn.
+        rewrite N.mod_small by (cbn; lia).
+        destruct flush; cbn; lia.
+      }
+      destruct flush; cbn; lia.
+    }
+    { easy. }
+    { reflexivity. }
+  Qed.
+
+End RealignerSpec.
 
