cava/Cava/Util/Byte.v
@@ -1,0 +1,217 @@
+(****************************************************************************)
+(* Copyright 2021 The Project Oak Authors                                   *)
+(*                                                                          *)
+(* Licensed under the Apache License, Version 2.0 (the "License")           *)
+(* you may not use this file except in compliance with the License.         *)
+(* You may obtain a copy of the License at                                  *)
+(*                                                                          *)
+(*     http://www.apache.org/licenses/LICENSE-2.0                           *)
+(*                                                                          *)
+(* Unless required by applicable law or agreed to in writing, software      *)
+(* distributed under the License is distributed on an "AS IS" BASIS,        *)
+(* WITHOUT WARRANTIES OR CONDITIONS OF ANY KIND, either express or implied. *)
+(* See the License for the specific language governing permissions and      *)
+(* limitations under the License.                                           *)
+(****************************************************************************)
+
+Require Import Coq.Arith.PeanoNat.
+Require Import Coq.Init.Byte.
+Require Import Coq.Lists.List.
+Require Import Coq.NArith.NArith.
+Require Import Coq.ZArith.ZArith.
+Require Import Coq.micromega.Lia.
+
+Require Import Cava.Util.List.
+Require Import Cava.Util.Nat.
+Require Import Cava.Util.Tactics.
+
+Require Import coqutil.Tactics.Tactics.
+
+Import ListNotations.
+
+(* Convert the least significant 8 bits of a number to a byte *)
+Definition N_to_byte (x : N) : byte :=
+  match Byte.of_N (x mod 2^8) with
+  | Some b => b
+  | None => x00
+  end.
+
+Module BigEndianBytes.
+  (* evaluate a big-endian list of bytes *)
+  Definition concat_bytes (bs : list byte) : N :=
+    List.fold_left (fun acc b => N.lor (N.shiftl acc 8) (Byte.to_N b)) bs 0%N.
+
+  (* convert the least significant (n*8) bits of a number to big-endian bytes *)
+  Definition N_to_bytes n (x : N) : list byte :=
+    List.map (fun i => N_to_byte (N.shiftr x (N.of_nat (n-1-i)*8)))
+             (seq 0 n).
+
+  (* convert a big-endian list of bytes to a list of n-byte words (length of list
+   must be a multiple of n) *)
+  Definition bytes_to_Ns n (x : list byte) : list N :=
+    List.map (fun i => concat_bytes (firstn n (skipn (n*i) x))) (seq 0 (length x / n)).
+End BigEndianBytes.
+
+Definition byte_xor (x y : byte) : byte := N_to_byte (N.lxor (Byte.to_N x) (Byte.to_N y)).
+
+Module N2Byte.
+  Lemma id (x: N) : ((Byte.to_N (N_to_byte x)) = x mod 256)%N.
+  Proof.
+    cbv [N_to_byte].
+    destr (Byte.of_N (x mod 2 ^ 8)).
+    { rewrite Byte.to_of_N with (x:=(x mod 2^8)%N) by apply E. reflexivity. }
+    { rewrite (Byte.of_N_None_iff (x mod 2^8))%N in E. exfalso.
+      pose (N.mod_upper_bound x (2^8))%N.
+      assert (2 ^ 8 <> 0)%N by (cbn;lia).
+      specialize (l H).
+      replace 255%N with (N.pred 256)%N in E by lia.
+      apply N.lt_pred_le in E.
+      apply N.lt_le_pred in l.
+      rewrite l in E.
+      cbn in E.
+      lia.
+    }
+  Qed.
+
+End N2Byte.
+
+Module Byte2N.
+  Lemma id x: (N_to_byte (Byte.to_N x) = x )%N.
+  Proof. destr x; now cbn. Qed.
+
+  Lemma inj x y: (Byte.to_N x = Byte.to_N y -> x = y)%N.
+  Proof.  intro H. rewrite <- (id x), <- (id y). now f_equal. Qed.
+End Byte2N.
+
+Section N.
+  Open Scope N.
+
+  Lemma testbit_byte b n:
+    (8 <= n) ->
+    N.testbit (Byte.to_N b) n = false.
+  Proof.
+    intros.
+    intros.
+    remember (Byte.to_N b) as b'.
+    pose (Byte.to_N_bounded b).
+    apply N.lt_succ_r in l.
+    change (N.succ 255) with (2^8) in l.
+    rewrite <- Heqb' in l.
+    apply N.testbit_high.
+    apply (N.lt_le_trans _ (2^8));
+      [ lia | apply N.pow_le_mono_r; lia ].
+  Qed.
+
+  Lemma unfold_N_to_bytes_4 x: BigEndianBytes.N_to_bytes 4 x =
+    [N_to_byte (N.shiftr x (N.of_nat (4 - 1 - 0) * 8));
+    N_to_byte (N.shiftr x (N.of_nat (4 - 1 - 1) * 8));
+    N_to_byte (N.shiftr x (N.of_nat (4 - 1 - 2) * 8));
+    N_to_byte (N.shiftr x (N.of_nat (4 - 1 - 3) * 8))].
+  Proof.
+    cbv [BigEndianBytes.N_to_bytes].
+    now cbn [List.map seq].
+  Qed.
+
+  Lemma shiftr_byte b x: (8 <= x) ->
+    N.shiftr (Byte.to_N b) x = 0.
+  Proof.
+    intros.
+    remember (Byte.to_N b) as b'.
+    pose (Byte.to_N_bounded b).
+    apply N.shiftr_eq_0.
+    apply N.lt_succ_r in l.
+    apply (N.lt_le_trans _ (N.log2 256)).
+    {
+      destr (0<?b').
+      2:{ destr (b'=?0); try rewrite E0; cbn; lia. }
+      apply N.log2_lt_pow2. { lia. }
+      cbn. now rewrite Heqb'.
+    }
+    now cbn.
+  Qed.
+End N.
+
+Lemma N_to_bytes_length n x : length (BigEndianBytes.N_to_bytes n x) = n.
+Proof. cbv [BigEndianBytes.N_to_bytes]. length_hammer. Qed.
+Hint Rewrite @N_to_bytes_length : push_length.
+
+Lemma bytes_to_Ns_length n bs :
+  length (BigEndianBytes.bytes_to_Ns n bs) = length bs / n.
+Proof. cbv [BigEndianBytes.bytes_to_Ns]. length_hammer. Qed.
+Hint Rewrite @bytes_to_Ns_length : push_length.
+
+Lemma N_to_byte_to_N x : Byte.to_N (N_to_byte x) = (x mod 256)%N.
+Proof.
+  cbv [N_to_byte]. change (2 ^ 8)%N with 256%N.
+  pose proof N.mod_bound_pos x 256 ltac:(lia) ltac:(lia).
+  pose proof proj1 (Byte.of_N_None_iff (x mod 256)).
+  apply Byte.to_of_N.
+  destruct (Byte.of_N (x mod 256)); [ reflexivity | ].
+  lazymatch goal with H : None = None -> _ |- _ =>
+                      specialize (H ltac:(reflexivity)) end.
+  lia.
+Qed.
+
+Lemma nth_bytes_to_Ns i n bs :
+  length bs mod n = 0 ->
+  n <> 0 ->
+  List.nth i (BigEndianBytes.bytes_to_Ns n bs) 0%N
+  = BigEndianBytes.concat_bytes
+      (List.map
+         (fun j => List.nth (i*n + j) bs Byte.x00)
+         (seq 0 n)).
+Proof.
+  cbv [BigEndianBytes.bytes_to_Ns]. intros.
+  destruct (Compare_dec.lt_dec i (length bs / n)).
+  { erewrite map_nth_inbounds with (d2:=0%nat) by length_hammer.
+    cbv [BigEndianBytes.concat_bytes]. f_equal; [ ].
+    push_nth. natsimpl.
+    erewrite firstn_map_nth with (d:=Byte.x00).
+    { eapply List.map_ext_in; intros *.
+      rewrite in_seq; natsimpl; intros.
+      push_nth. f_equal; lia. }
+    { push_length.
+      Zify.zify.
+      (* extra step because zify fails to zify Nat.modulo and Nat.div *)
+      rewrite ?mod_Zmod, ?div_Zdiv in * by lia.
+      Zify.zify; Z.to_euclidean_division_equations.
+      (* N.B. this needs nia instead of lia *)
+      nia. } }
+  { push_nth. cbv [BigEndianBytes.concat_bytes].
+    assert (length bs <= i * n).
+    { Zify.zify.
+      (* extra step because zify fails to zify Nat.modulo and Nat.div *)
+      rewrite ?mod_Zmod, ?div_Zdiv in * by lia.
+      Zify.zify; Z.to_euclidean_division_equations.
+      (* N.B. this needs nia instead of lia *)
+      nia. }
+    apply fold_left_invariant with (I:= eq 0%N); [ reflexivity | | tauto ].
+    intros *; rewrite in_map_iff.
+    intros; logical_simplify; subst.
+    match goal with H : _ |- _ => apply in_seq in H end.
+    push_nth. reflexivity. }
+Qed.
+
+Lemma N_to_byte_equiv x y :
+  (x mod 256 = y mod 256)%N -> N_to_byte x = N_to_byte y.
+Proof.
+  intro Heq. cbv [N_to_byte]. compute_expr (2 ^ 8)%N.
+  rewrite Heq. reflexivity.
+Qed.
+
+Lemma nth_N_to_bytes i n x :
+  i < n ->
+  List.nth i (BigEndianBytes.N_to_bytes n x) Byte.x00
+  = N_to_byte (N.shiftr (N.land x (N.ones (8 * N.of_nat n)))
+                        (N.of_nat (n - 1 - i) * 8)).
+Proof.
+  intros. cbv [BigEndianBytes.N_to_bytes].
+  push_nth; natsimpl. apply N_to_byte_equiv.
+  change 256%N with (2 ^ 8)%N.
+  apply N.bits_inj; intro j.
+  push_Ntestbit; boolsimpl.
+  case_eq (j <? 8)%N; intros; N.bool_to_prop; [ | reflexivity ].
+  push_Ntestbit. boolsimpl.
+  f_equal; lia.
+Qed.
+
